Progress on an 'echo' div example

examples/divScript.sml
@@ -121,18 +121,40 @@ QED
 
 (* A small IO model needed for IO examples *)
 
-val names_def = Define `names = ["put_char"]`;
+val names_def = Define `names = ["put_char"; "get_char"]`;
 
 val put_char_event_def = Define `
   put_char_event c = IO_event "put_char" [n2w (ORD c)] []`;
 
+val get_char_event_def = Define `
+  get_char_event c = IO_event "get_char" [] [0w, 1w; 0w, n2w (ORD c)]`;
+
+val get_char_eof_event_def = Define `
+  get_char_eof_event = IO_event "get_char" [] [0w, 0w; 0w, 0w]`;
+
 val update_def = Define `
-  update "put_char" [c] [] s = case destStr s of
-    | NONE     => NONE
-    | SOME out => SOME (FFIreturn [] (Str (SNOC (CHR (w2n c)) out)))`
+  (update "put_char" [c] [] s = case destCons s of
+     | NONE                 => NONE
+     | SOME (input, output) => case destStr output of
+       | NONE   => NONE
+       | SOME l => SOME (FFIreturn []
+         (Cons input (Str (SNOC (CHR (w2n c)) l))))) /\
+  (update "get_char" [] [0w; 0w] s = case destCons s of
+     | NONE                 => NONE
+     | SOME (input, output) => case destStream input of
+       | NONE    => NONE
+       | SOME ll => if ll = [||] then
+           SOME (FFIreturn [0w; 0w] s)
+         else
+           SOME (FFIreturn [1w; n2w (THE (LHD ll))]
+                           (Cons (Stream (THE (LTL ll))) output)))`
+
+val State_def = Define `
+  State input output = Cons (Stream (LMAP ORD input)) (Str output)`
 
 val SIO_def = Define `
-  SIO out events = one (FFI_part (Str out) update names events)`
+  SIO input output events =
+    one (FFI_part (State input output) update names events)`
 
 val _ = process_topdecs `
   fun put_char c = let
@@ -142,33 +164,85 @@ val _ = process_topdecs `
     in () end
   ` |> append_prog;
 
+val _ = process_topdecs `
+  fun get_char (u:unit) = let
+      val a = Word8Array.array 2 (Word8.fromInt 0)
+      val _ = #(get_char) "" a
+    in if Word8Array.sub a 0 = Word8.fromInt 1 then
+        Some (Char.chr (Word8.toInt (Word8Array.sub a 1)))
+      else
+        None
+    end
+  ` |> append_prog;
+
 val st = ml_translatorLib.get_ml_prog_state();
 
 Theorem put_char_spec:
-  !c cv s events.
+  !c cv input output events.
   limited_parts names p /\ CHAR c cv ==>
   app (p:'ffi ffi_proj) ^(fetch_v "put_char" st) [cv]
-    (SIO s events)
+    (SIO input output events)
     (POSTv v. &UNIT_TYPE () v *
-              SIO (SNOC c s) (SNOC (put_char_event c) events))
+              SIO input (SNOC c output) (SNOC (put_char_event c) events))
 Proof
   xcf "put_char" st
   \\ xlet_auto THEN1 (xcon \\ xsimpl)
   \\ xlet_auto THEN1 (xcon \\ xsimpl)
-  \\ xlet `POSTv v. &STRING_TYPE (implode [c]) v * SIO s events`
+  \\ xlet
+    `POSTv v. &STRING_TYPE (implode [c]) v * SIO input output events`
   THEN1 (xapp \\ xsimpl \\ qexists_tac `[c]` \\ fs [LIST_TYPE_def])
   \\ xlet_auto THEN1 xsimpl
   \\ xlet_auto THEN1 xsimpl
   \\ rename1 `W8ARRAY av`
-  \\ xlet `POSTv v. &UNIT_TYPE () v * W8ARRAY av [] *
-                    SIO (SNOC c s) (SNOC (put_char_event c) events)`
+  \\ xlet
+    `POSTv v. &UNIT_TYPE () v * W8ARRAY av [] *
+              SIO input (SNOC c output) (SNOC (put_char_event c) events)`
   THEN1 (
-    xffi \\ xsimpl
+    xffi \\ xsimpl \\ fs [SIO_def]
     \\ MAP_EVERY qexists_tac
-      [`[n2w (ORD c)]`, `emp`, `Str s`, `update`, `names`, `events`]
-    \\ fs [SIO_def, update_def, put_char_event_def, names_def,
-           SNOC_APPEND, implode_def, STRING_TYPE_def] \\ xsimpl)
+      [`[n2w (ORD c)]`, `emp`, `State input output`, `update`, `names`,
+       `events`]
+    \\ fs [update_def, put_char_event_def, names_def, SNOC_APPEND,
+           implode_def, STRING_TYPE_def, State_def]
+    \\ xsimpl)
   \\ xcon \\ xsimpl
+QED
+
+Theorem get_char_spec:
+  !uv c input output events.
+  limited_parts names p /\ UNIT_TYPE () uv ==>
+  app (p:'ffi ffi_proj) ^(fetch_v "get_char" st) [uv]
+    (SIO input output events)
+    (POSTv v. &OPTION_TYPE CHAR (LHD input) v *
+              if input = [||] then
+                SIO input output (SNOC (get_char_eof_event) events)
+              else
+                SIO (THE (LTL input)) output
+                    (SNOC (get_char_event (THE (LHD input))) events))
+Proof
+  xcf "get_char" st
+  \\ qmatch_goalsub_abbrev_tac `_ * sio`
+  \\ qabbrev_tac `a:word8 list = if input = [||] then
+                                   [0w; 0w]
+                                 else
+                                   [1w; n2w (ORD (THE (LHD input)))]`
+  \\ xmatch \\ rpt (xlet_auto THEN1 xsimpl)
+  \\ Cases_on `input` \\ (
+    fs [] \\ rename1 `W8ARRAY av`
+    \\ xlet `POSTv v. &UNIT_TYPE () v * W8ARRAY av a * sio`
+    THEN1 (
+      xffi \\ xsimpl \\ fs [SIO_def]
+      \\ qpat_abbrev_tac `s = State _ _`
+      \\ MAP_EVERY qexists_tac [`emp`, `s`, `update`, `names`, `events`]
+      \\ unabbrev_all_tac
+      \\ fs [update_def, get_char_event_def, get_char_eof_event_def,
+             names_def, SNOC_APPEND, EVAL ``REPLICATE 2 0w``, State_def]
+      \\ xsimpl)
+    \\ rpt (xlet_auto THEN1 xsimpl)
+    \\ xlet_auto THEN1 (xsimpl \\ fs [WORD_def])
+    \\ xif \\ instantiate
+    \\ rpt (xlet_auto THEN1 xsimpl)
+    \\ xcon \\ xsimpl \\ fs [OPTION_TYPE_def, CHR_ORD, ORD_BOUND])
 QED
 
 (* Useful definitions *)
@@ -218,25 +292,36 @@ Theorem printLoop_spec:
   !c cv.
     limited_parts names p /\ CHAR c cv ==>
     app (p:'ffi ffi_proj) ^(fetch_v "printLoop" st) [cv]
-      (SIO "" []) (POSTd io. io = LREPEAT [put_char_event c])
+      (SIO [||] "" []) (POSTd io. io = LREPEAT [put_char_event c])
 Proof
   xcf_div "printLoop" st
   \\ MAP_EVERY qexists_tac
-    [`K emp`, `\i. REPLICATE [put_char_event c] i`, `K($= cv)`,
-     `\i. Str (REPLICATE [c] i)`, `update`]
+    [`K emp`, `\i. REPLICATE [put_char_event c] i`, `K ($= cv)`,
+     `\i. State [||] (REPLICATE [c] i)`, `update`]
   \\ fs [GSYM SIO_def, REPLICATE_def]
   \\ xsimpl \\ rw [lprefix_lub_def]
   THEN1 (
     xlet `POSTv v. &UNIT_TYPE () v *
-                   SIO (REPLICATE [c] (SUC i))
+                   SIO [||] (REPLICATE [c] (SUC i))
                        (REPLICATE [put_char_event c] (SUC i))`
     THEN1 (
       xapp
       \\ MAP_EVERY qexists_tac
-        [`emp`, `REPLICATE [c] i`, `REPLICATE [put_char_event c] i`, `c`]
+        [`emp`, `REPLICATE [c] i`, `[||]`,
+         `REPLICATE [put_char_event c] i`, `c`]
       \\ fs [REPLICATE_SNOC] \\ xsimpl)
     \\ xvar \\ fs [REPLICATE_APPEND] \\ xsimpl)
   THEN1 fs [LPREFIX_REPLICATE_LREPEAT]
+
+(* alternative version using REPLICATE_LREPEAT
+  \\ fs [PULL_EXISTS]
+  \\ qmatch_goalsub_abbrev_tac `LPREFIX ll`
+  \\ `ub = ll` suffices_by simp []
+  \\ unabbrev_all_tac
+  \\ irule REPLICATE_LREPEAT
+  \\ fs []
+*)
+
   \\ qmatch_goalsub_abbrev_tac `LPREFIX a1 a2`
   \\ `a1 = a2` suffices_by simp[]
   \\ unabbrev_all_tac
@@ -266,6 +351,150 @@ Proof
   \\ simp[LPREFIX_LCONS]
   \\ rw[]
   \\ rw[LTL_LCONS]
+QED
+
+(* An IO-conditional loop with side effects *)
+
+val _ = process_topdecs `
+  fun echoLoop (u:unit) = case get_char () of
+      None   => ()
+    | Some c => (put_char c; echoLoop ());
+  ` |> append_prog;
+
+val st = ml_translatorLib.get_ml_prog_state();
+
+val echo_def = Define `
+  echo l = FLAT (MAP (\c. [get_char_event c; put_char_event c]) l)`
+
+val lecho_def = Define `
+  lecho ll = LFLATTEN (LMAP (\c. fromList [get_char_event c;
+                                          put_char_event c]) ll)`
+
+Theorem lecho_LTAKE_SUC:
+  !ll c n.
+    LNTH n ll = SOME c ==>
+    THE (LTAKE (2 * SUC n) (lecho ll)) =
+      THE (LTAKE (2 * n) (lecho ll)) ++
+        [get_char_event c; put_char_event c]
+Proof
+  cheat
+QED
+
+Theorem echoLoop_spec:
+  !uv input.
+    limited_parts names p /\ UNIT_TYPE () uv ==>
+    app (p:'ffi ffi_proj) ^(fetch_v "echoLoop" st) [uv]
+      (SIO input "" []) (POSTvd
+        (\v. &(LFINITE input /\ UNIT_TYPE () v) *
+             SIO [||] (THE (toList input))
+                 (SNOC get_char_eof_event (echo (THE (toList input)))))
+        (\io. ~LFINITE input /\ io = lecho input))
+Proof
+  rw [] \\ Cases_on `LFINITE input` \\ fs [POSTvd_def, SEP_CLAUSES]
+  \\ fs [SEP_F_to_cond, GSYM POSTv_def, GSYM POSTd_def]
+  THEN1 (
+    reverse (sg `
+      (\input.
+         !uv output events.
+           app p echoLoop_v [uv] (SIO input output events)
+             (POSTv v. &UNIT_TYPE () v *
+                       SIO [||] (output ++ THE (toList input))
+                           (events ++ SNOC get_char_eof_event
+                                           (echo (THE (toList input))))))
+        input`)
+    THEN1 (
+      fs [] \\ pop_assum (qspecl_then [`uv`, `[]`, `[]`] mp_tac) \\ fs [])
+    \\ irule LFINITE_STRONG_INDUCTION \\ rw []
+    THEN1 (
+      xcf "echoLoop" st
+      \\ xmatch
+      \\ xlet_auto THEN1 (xcon \\ xsimpl)
+      \\ xlet `POSTv v. &OPTION_TYPE CHAR NONE v *
+                        SIO [||] output
+                            (SNOC (get_char_eof_event) events)`
+      THEN1 (
+        xapp
+        \\ MAP_EVERY qexists_tac [`emp`, `output`, `[||]`, `events`]
+        \\ xsimpl)
+      \\ xmatch \\ fs [OPTION_TYPE_def]
+      \\ reverse (rw []) THEN1 EVAL_TAC
+      \\ xcon \\ fs [toList, echo_def, SNOC_APPEND] \\ xsimpl)
+    \\ xcf "echoLoop" st
+    \\ xmatch
+    \\ xlet_auto THEN1 (xcon \\ xsimpl)
+    \\ xlet `POSTv v. &OPTION_TYPE CHAR (SOME h) v *
+                      SIO t output (SNOC (get_char_event h) events)`
+    THEN1 (
+      xapp
+      \\ MAP_EVERY qexists_tac [`emp`, `output`, `h ::: t`, `events`]
+      \\ xsimpl)
+    \\ xmatch \\ fs [OPTION_TYPE_def] \\ reverse (rpt strip_tac)
+    THEN1 EVAL_TAC THEN1 EVAL_TAC
+    \\ xlet `POSTv v. &UNIT_TYPE () v *
+                      SIO t (SNOC h output)
+                          (SNOC (put_char_event h)
+                                (SNOC (get_char_event h) events))`
+    THEN1 (xapp \\ fs [])
+    \\ xlet_auto THEN1 (xcon \\ xsimpl)
+    \\ qmatch_goalsub_abbrev_tac `SIO _ output1 events1`
+    \\ qmatch_goalsub_abbrev_tac `_ * SIO _ output2 events2`
+    \\ `output2 = output1 ++ THE (toList t)` by (
+      unabbrev_all_tac \\ drule LFINITE_HAS_LENGTH \\ strip_tac
+      \\ drule LTAKE_LLENGTH_SOME \\ strip_tac \\ fs [toList])
+    \\ `events2 = events1 ++ SNOC get_char_eof_event
+                                  (echo (THE (toList t)))` by (
+      unabbrev_all_tac \\ fs [SNOC_APPEND, echo_def])
+    \\ xapp
+    \\ MAP_EVERY qexists_tac [`emp`, `output1`, `events1`]
+    \\ xsimpl)
+  \\ xcf_div "echoLoop" st
+  \\ MAP_EVERY qexists_tac
+    [`K emp`, `\i. THE (LTAKE (2 * i) (lecho input))`, `K ($= uv)`,
+     `\i. State (THE (LDROP i input)) (THE (LTAKE i input))`, `update`]
+  \\ fs [GSYM SIO_def] \\ xsimpl \\ rw [lprefix_lub_def]
+  THEN1 (
+    qmatch_goalsub_abbrev_tac `SIO input1 output1 events1`
+    \\ qmatch_goalsub_abbrev_tac `&_ * _ * SIO input2 output2 events2`
+    \\ Cases_on `LNTH i input` THEN1 metis_tac [LFINITE_LNTH_NONE]
+    \\ rename1 `LNTH _ _ = SOME c`
+    \\ `input1 = c ::: input2` by (
+      Cases_on `LDROP i input` \\ Cases_on `LDROP (SUC i) input`
+      \\ TRY (metis_tac [LDROP_NONE_LFINITE])
+      \\ unabbrev_all_tac \\ qabbrev_tac `input2 = LDROP (SUC i) input`
+      \\ drule NOT_LFINITE_DROP_LFINITE \\ disch_then drule
+      \\ drule LNTH_LDROP \\ fs []
+      \\ rpt strip_tac \\ unabbrev_all_tac \\ rename1 `ll = _`
+      \\ Cases_on `ll` \\ fs [SUC_ONE_ADD, LDROP_ADD] \\ rfs [])
+    \\ `output2 = SNOC c output1` by (
+      Cases_on `LTAKE i input` \\ Cases_on `LTAKE (SUC i) input`
+      \\ TRY (metis_tac [LFINITE])
+      \\ unabbrev_all_tac
+      \\ drule LTAKE_LNTH_EL \\ disch_then (qspec_then `i` mp_tac)
+      \\ strip_tac \\ fs [LTAKE_SNOC_LNTH] \\ rfs [])
+    \\ xmatch
+    \\ xlet_auto THEN1 (xcon \\ xsimpl)
+    \\ xlet `POSTv v. &OPTION_TYPE CHAR (SOME c) v *
+                      SIO input2 output1
+                          (SNOC (get_char_event c) events1)`
+    THEN1 (
+      xapp
+      \\ MAP_EVERY qexists_tac [`emp`, `output1`, `input1`, `events1`]
+      \\ xsimpl)
+    \\ xmatch \\ fs [OPTION_TYPE_def] \\ reverse (rpt strip_tac)
+    THEN1 EVAL_TAC THEN1 EVAL_TAC
+    \\ xlet `POSTv v. &UNIT_TYPE () v * SIO input2 output2 events2`
+    THEN1 (
+      xapp
+      \\ MAP_EVERY qexists_tac [`emp`, `output1`, `input2`,
+                                `SNOC (get_char_event c) events1`, `c`]
+      \\ qmatch_goalsub_abbrev_tac `&_ * SIO _ _ events'`
+      \\ `events' = events2` by (
+        unabbrev_all_tac \\ fs [SNOC_APPEND, lecho_LTAKE_SUC])
+      \\ fs [SNOC_APPEND] \\ xsimpl)
+    \\ xlet_auto THEN1 (xcon \\ xsimpl)
+    \\ xvar \\ fs [SNOC_APPEND, UNIT_TYPE_def] \\ xsimpl)
+  THEN1 cheat
+  \\ cheat
 QED
 
 val _ = export_theory();
